src/coq/Handlers/Handlers.v
@@ -26,7 +26,6 @@ From Vellvm.Handlers Require Export
      FiniteMemory
      FiniteMemoryTheory
      Pick
-     UndefinedBehaviour
      OOM
      Serialization.
 
